src/Hoare.v
@@ -1,5 +1,6 @@
+Require Import Mem.
 Require Import Prog.
-Require Import Pred.
+Require Import Pred PredCrash.
 Require Import List.
 Require Import Morphisms.
 Require Import Word.
